Restore and upgrade UFCMA

src/tls/HMAC.UFCMA.fst
@@ -13,11 +13,11 @@ module MM = FStar.Monotonic.Map
 
 // To be moved to Flags.
 let model = Flags.model
-assume val ideal: b:bool{b ==> model}
+private assume val ideal: b:bool{b ==> model}
 let ipkg = Pkg.ipkg
 type safe (#ip:ipkg) (i:ip.Pkg.t) = ideal /\ ip.Pkg.honest i
 
-let is_safe (#ip:ipkg) (i:ip.Pkg.t{ip.Pkg.registered i})
+private let is_safe (#ip:ipkg) (i:ip.Pkg.t{ip.Pkg.registered i})
   : ST bool (requires fun h0 -> True)
   (ensures fun h0 b h1 -> modifies_none h0 h1 /\ (b <==> safe i))
   =
@@ -42,10 +42,7 @@ let keylen (u:info): Pkg.keylen = UInt32.uint_to_t (Hashing.Spec.tagLen u.alg)
 type keyrepr (u:info) = Hashing.Spec.hkey u.alg
 
 let goodish (#ip:ipkg) (i:ip.Pkg.t) (u:info) (msg:text) =
-  _: unit{
-  (~ ideal)\/
-  ip.Pkg.corrupt i \/
-  u.good msg}
+  _: unit{~(safe i) \/ u.good msg}
 
 private type log_t
   (#ip:ipkg)
@@ -67,34 +64,40 @@ noeq abstract type ir_key (ip:ipkg) (i:ip.Pkg.t) =
     ir_key ip i
   | RealKey: ck:concrete_key -> ir_key ip i
 
-type key (ip:ipkg) (i:ip.Pkg.t) =
+type key (ip:ipkg) (i:ip.Pkg.t{ip.Pkg.registered i}) =
   (if model then
     k:ir_key ip i{IdealKey? k <==> safe i}
   else concrete_key)
 
-let usage (#ip:ipkg) (#i:ip.Pkg.t) (k:key ip i) : GTot info =
+let usage (#ip:ipkg) (#i:ip.Pkg.t{ip.Pkg.registered i}) (k:key ip i) : GTot info =
   if model then
     match k <: ir_key ip i with
     | IdealKey ck _ _ -> ck.u
     | RealKey ck -> ck.u
   else k.u
 
-let keyval (#ip:ipkg) (#i:ip.Pkg.t) (k:key ip i) : GTot (keyrepr (usage k)) =
+let keyval (#ip:ipkg) (#i:ip.Pkg.t{ip.Pkg.registered i}) (k:key ip i)
+  : GTot (keyrepr (usage k)) =
   if model then
     match k <: ir_key ip i with
     | IdealKey ck _ _ -> ck.k
     | RealKey ck -> ck.k
   else k.k
 
-let region (#ip:ipkg) (#i:ip.Pkg.t) (k:key ip i)
+let region (#ip:ipkg) (#i:ip.Pkg.t{ip.Pkg.registered i}) (k:key ip i)
   : Ghost (subrgn (usage k).parent)
   (requires safe i) (ensures fun _ -> True)
   = let IdealKey _ r _ = k <: ir_key ip i in r
 
-let footprint (#ip:ipkg) (#i:ip.Pkg.t {ip.Pkg.registered i}) (k:key ip i) : Pkg.rset =
+let shared_footprint : rset = Set.empty
+
+let footprint (#ip:ipkg) (#i:ip.Pkg.t {ip.Pkg.registered i}) (k:key ip i)
+  : s:rset{s `Set.disjoint` shared_footprint}
+  =
+  assume false; // FIXME downwards closed set
   if model then
     match k <: ir_key ip i with
-    | IdealKey _ r _ -> assume false; Set.singleton r // FIXME downwards closed set
+    | IdealKey _ r _ -> Set.singleton r
     | RealKey _ -> Set.empty
   else Set.empty
 
@@ -109,64 +112,36 @@ val create:
     Pkg.fresh_regions (footprint k) h0 h1)
 
 let create ip _ _ i u =
-  let region: Mem.subrgn u.parent = new_region u.parent in
-  assert(~(is_tls_rgn u.parent));
-  let log: log_t #ip i u region = MM.alloc #_ #_ #_ #_ in
   let kv: keyrepr u = CoreCrypto.random (Hashing.Spec.tagLen u.alg) in
-<<<<<<< HEAD
-  gen ip i u kv 
-
-// placeholder; will require allocating the sub-region only ideally.
-assume val coerceT: 
-  ip: ipkg -> ha_of_i: (ip.Pkg.t -> ha) -> good_of_i: (ip.Pkg.t -> text -> bool) ->
-  i: ip.Pkg.t {ip.Pkg.registered i} -> 
-  u: (u: info {u.alg = ha_of_i i /\ u.good == good_of_i i}) ->
-  kv: Pkg.lbytes (keylen u) -> 
-  key ip i
-
-val coerce: 
-=======
   let ck = MAC u kv in
   let k : ir_key ip i =
     if is_safe i then
+      let region: Mem.subrgn u.parent = new_region u.parent in
+      assert(~(is_tls_rgn u.parent));
+      let log: log_t #ip i u region = MM.alloc #_ #_ #_ #_ in
       IdealKey ck region log
     else
       RealKey ck in
   k <: key ip i
 
 let coerceT (ip: ipkg) (ha_of_i: ip.Pkg.t -> ha) (good_of_i: ip.Pkg.t -> text -> bool)
-  (i: ip.Pkg.t {ip.Pkg.registered i}) (u: u:info {u.alg = ha_of_i i /\ u.good == good_of_i i})
-  (kv: Pkg.lbytes (keylen u))
-  : Ghost (key ip i) (requires ~(safe i)) (ensures fun _ -> True) =
+  (i: ip.Pkg.t {ip.Pkg.registered i /\ ~(safe i)}) (u: u:info {u.alg = ha_of_i i /\ u.good == good_of_i i})
+  (kv: Pkg.lbytes (keylen u)) : GTot (key ip i)
+  =
   let ck = MAC u kv in
   if model then
     let k : ir_key ip i = RealKey ck in k
   else ck
 
 val coerce:
->>>>>>> Checkpoint
   ip: ipkg -> ha_of_i: (ip.Pkg.t -> ha) -> good_of_i: (ip.Pkg.t -> text -> bool) ->
-  i: ip.Pkg.t {ip.Pkg.registered i} ->
+  i: ip.Pkg.t {ip.Pkg.registered i /\ ~(safe i)} ->
   u: (u: info {u.alg = ha_of_i i /\ u.good == good_of_i i}) ->
   kv: Pkg.lbytes (keylen u) ->
   ST (k:key ip i)
-<<<<<<< HEAD
-  (requires (fun _ -> ideal ==> ip.Pkg.corrupt i))
-  (ensures (fun h0 k h1 ->
-    modifies Set.empty h0 h1 /\
-    k == coerceT ip ha_of_i good_of_i i u kv /\
-    k.u == u /\
-    fresh_subregion (region k) u.parent h0 h1 ))
-let coerce ip ha_of_i good_of_i i u kv = 
-  let k = gen ip i u kv in
-  assume (k == coerceT ip ha_of_i good_of_i i u kv);
-  k
-
-=======
-  (requires fun _ -> ~(safe i))
+  (requires fun _ -> True)
   (ensures fun h0 k h1 ->
     modifies_none h0 h1 /\
-    ~(safe i) /\ // annoying
     k == coerceT ip ha_of_i good_of_i i u kv /\
     usage k == u /\
     Pkg.fresh_regions (footprint k) h0 h1)
@@ -176,103 +151,54 @@ let coerce ip _ _ i u kv =
   if model then
     let k : ir_key ip i = RealKey ck in k
   else ck
->>>>>>> Checkpoint
 
 // not quite doable without reification?
 // assert_norm(forall ip i u. (create #ip i u == coerce #ip i u (CoreCrypto.random (UInt32.v (keylen u)))))
 
-unfold let info1
-  (ip:ipkg)
-  (ha_of_i: ip.Pkg.t -> ha)
-  (good_of_i: ip.Pkg.t -> text -> bool)
-  (i: ip.Pkg.t): Type0
+private let get_key (#ip:ipkg) (#i:ip.Pkg.t{ip.Pkg.registered i}) (k:key ip i)
+  : concrete_key
   =
-  a:info{a.alg = ha_of_i i /\ a.good == good_of_i i}
-
-unfold let localpkg
-  (ip: ipkg)
-  (ha_of_i: i:ip.Pkg.t -> ha)
-<<<<<<< HEAD
-  (good_of_i: ip.Pkg.t -> text -> bool) 
-  : 
-  p: Pkg.local_pkg ip {Pkg.LocalPkg?.info #ip p == info1 ip ha_of_i good_of_i}
-= 
-=======
-  (good_of_i: ip.Pkg.t -> text -> bool)
-  : p: Pkg.local_pkg ip {Pkg.LocalPkg?.info #ip p == info1 ip ha_of_i good_of_i}
-  =
->>>>>>> Checkpoint
-    Pkg.LocalPkg
-      (fun (i:ip.Pkg.t {ip.Pkg.registered i}) -> key ip i)
-      (info1 ip ha_of_i good_of_i)
-      (fun #_ u -> keylen u )
-      ideal
-      footprint // local footprint
-      (fun #_ k h -> True) // local invariant
-      (fun r i h0 k h1 -> ()) // Local invariant framing
-      (fun #i u k h1 -> usage k == u) // create/coerce postcondition
-      (fun #i u k h1 r h2 -> ())
-      (create ip ha_of_i good_of_i)
-      (coerceT ip ha_of_i good_of_i)
-      (coerce ip ha_of_i good_of_i)
-
-unfold
-let pkg
-  (ip:ipkg)
-  (ha_of_i: ip.Pkg.t -> ha)
-  (good_of_i: ip.Pkg.t -> text -> bool)
-  (table: Pkg.mem_table (key ip))
-  : Pkg.pkg ip
-//  (requires fun h0 -> True)
-//  (ensures fun h0 r h1 -> modifies_one tls_define_region h0 h1)
-=
-  let p = localpkg ip ha_of_i good_of_i in
-  //assert(p.Pkg.key == key ip);
-  assert(Pkg.LocalPkg?.info #ip p == info1 ip ha_of_i good_of_i);
-
-  let table: Pkg.mem_table p.Pkg.key = admit() in //table in
-  let q = Pkg.memoization p table in
-  assert(Pkg.Pkg?.key q == key ip);
-  q
-
-val leak:
-  #ip: ipkg ->
-  #i: ip.Pkg.t ->
-  k: key ip i {ip.Pkg.corrupt i} -> kv:keyrepr k.u { kv = keyval k }
-let leak #_ #_ k = k.kv
+  if model then
+    (match k <: ir_key ip i with
+    | IdealKey rk _ _ -> rk
+    | RealKey rk -> rk)
+  else k
 
 val mac:
-  #ip:ipkg -> #i:ip.Pkg.t -> k:key ip i ->
-  p:text {ip.Pkg.corrupt i \/ k.u.good p} -> ST (tag k.u)
-  (requires (fun _ -> True))
-  (ensures (fun h0 t h1 -> modifies (Set.singleton (region k)) h0 h1 ))
+  #ip:ipkg -> #i:ip.Pkg.t{ip.Pkg.registered i} -> k:key ip i ->
+  p:text {(usage k).good p \/ ~(safe i)} ->
+  ST (tag (usage k))
+  (requires fun _ -> True)
+  (ensures fun h0 t h1 -> modifies (footprint k) h0 h1)
   // we may be more precise to prove ideal functional correctness,
   // e,g,  /\ sel h1 k.log = snoc (sel h0 k.log) (Entry t p)
+
 let mac #ip #i k p =
-  let kv: keyrepr k.u = k.kv in
-  let t: tag k.u = HMAC.hmac k.u.alg kv p in
-  if None? (MM.lookup k.log (t,p)) then MM.extend k.log (t,p) ();
+  let MAC u kv = get_key k in
+  let t = HMAC.hmac u.alg kv p in
+  (if is_safe i then
+    (let IdealKey _ _ log = k <: ir_key ip i in
+    if None? (MM.lookup log (t, p)) then MM.extend log (t,p) ()));
   t
 
 val verify:
   #ip:ipkg -> #i:ip.Pkg.t {ip.Pkg.registered i} -> k:key ip i ->
-  p:text -> t: tag k.u -> ST bool
-  (requires (fun _ -> True))
-  (ensures (fun h0 b h1 ->
-    modifies Set.empty h0 h1 /\
-    (b /\ ideal /\ ip.Pkg.honest i ==> k.u.good p)))
+  p:text -> t: tag (usage k) ->
+  ST bool
+  (requires fun _ -> True)
+  (ensures fun h0 b h1 -> modifies_none h0 h1 /\
+    (b /\ safe i ==> (usage k).good p))
 
 // We use the log to correct any verification errors
 let verify #ip #i k p t =
-  let verified = HMAC.hmacVerify k.u.alg k.kv p t in
-  if ideal then
-    let bad = not(ip.Pkg.get_honesty i) in
-    match FStar.Monotonic.Map.lookup k.log (t,p) with
-    | Some _ -> verified        (* genuine MAC *)
-    | None   -> verified && bad (* forgery, blocked when ideal & honest *)
+  let MAC u kv = get_key k in
+  let verified = HMAC.hmacVerify u.alg kv p t in
+  if is_safe i then
+    let IdealKey _ _ log = k <: ir_key ip i in
+    let valid = Some? (MM.lookup log (t,p)) in
+    verified && valid
   else
     verified
-
 
 /// Now entirely independent of TLS.
 ///
@@ -287,6 +213,29 @@ let verify #ip #i k p t =
 /// - how to deal with agility here?
 /// - which level of abstraction?
 
+type info1 (ip:ipkg) (ha_of_i: ip.Pkg.t -> ha)
+  (good_of_i: ip.Pkg.t -> text -> bool) (i: ip.Pkg.t)
+  =
+  a:info{a.alg = ha_of_i i /\ a.good == good_of_i i}
+
+unfold let localpkg (ip: ipkg) (ha_of_i: i:ip.Pkg.t -> ha) (good_of_i: ip.Pkg.t -> text -> bool)
+  : Pure (Pkg.local_pkg ip)
+  (requires True) (ensures fun p -> p.Pkg.key == key ip /\ p.Pkg.info == info1 ip ha_of_i good_of_i)
+  =
+  Pkg.LocalPkg
+    (key ip)
+    (info1 ip ha_of_i good_of_i)
+    (fun #_ u -> keylen u )
+    ideal
+    shared_footprint
+    footprint // local footprint
+    (fun #_ k h -> True) // local invariant
+    (fun r i h0 k h1 -> ()) // Local invariant framing
+    (fun #i u k h1 -> usage k == u) // create/coerce postcondition
+    (fun #i u k h1 r h2 -> ())
+    (create ip ha_of_i good_of_i)
+    (coerceT ip ha_of_i good_of_i)
+    (coerce ip ha_of_i good_of_i)
 
 /// TODOs:
 /// - Type0/Type1
@@ -295,44 +244,37 @@ let verify #ip #i k p t =
 /// - more specific instantiations?
 /// (later) support dynamic key compromise
 
-val coerce_eq2: a: (nat -> Type0) -> b: (nat -> Type0) -> v:a 0{a == b} -> b 0
-let coerce_eq2 a b v = v // this works; many similar variants did not.
+val coerce_eq2: a: (nat -> Type0) -> b: (nat -> Type0) -> v:a 0 -> Pure (b 0)
+  (requires a == b) (ensures fun _ -> True)
+let coerce_eq2 _ _ v = v // this works; many similar variants did not.
 
 module MR = FStar.Monotonic.RRef
 
-#set-options "--initial_fuel 1 --max_fuel 3 --initial_ifuel 1 --max_ifuel 3"
+#set-options "--initial_fuel 1 --max_fuel 4 --initial_ifuel 1 --max_ifuel 4"
 open FStar.Tactics
 
-let test
-  (r:rgn {~(is_tls_rgn r)})
-  (v': bytes)
-  (t': Hashing.Spec.tag Hashing.SHA256)
-  :
-  ST unit
-  (requires fun h0 -> Pkg.model)
-  (ensures fun h0 _ h1 -> True)
-=
-  let ip = Pkg.Idx // honest, simple indexes
-    nat
-    (fun _ -> True)
-    (fun _ -> True)
-    (fun _ -> False)
-    (fun _ -> true) in
+type id = nat
+let ip : ipkg = Pkg.Idx id (fun _ -> True) (fun _ -> True) (fun _ -> true)
 
+let test (r:rgn {~(is_tls_rgn r)}) (v': bytes) (t': Hashing.Spec.tag Hashing.SHA256)
+  : ST unit
+  (requires fun h0 -> model)
+  (ensures fun h0 _ h1 -> True)
+  =
   // testing usability of local packages
   let a = Hashing.SHA256 in
-  let ha_of_i (i:nat) = a in
-  let good_of_i i v = length v = i in // a property worth MACing!
+  let ha_of_i (i:ip.Pkg.t) = a in
+  let good_of_i (i:ip.Pkg.t) (v:text) = length v = 0 in // a property worth MACing!
+
   let p = localpkg ip ha_of_i good_of_i in
-  // assert (Pkg.LocalPkg?.info #ip p == info1 ip ha_of_i good_of_i); // provable only with unfolds?
+  let table = mem_alloc (key ip) in
+  let q = Pkg.memoization p table in
 
-  let u = {parent=r; alg=a; good=good_of_i 0} in
-  let u = coerce_eq2 (info1 ip ha_of_i good_of_i) (Pkg.LocalPkg?.info #ip p) u in
-  let k0: key ip 0 = (Pkg.LocalPkg?.create p) 0 u in
+  assert(Pkg.Pkg?.key q == key ip);
+  assert(Pkg.Pkg?.info q == info1 ip ha_of_i good_of_i);
 
-  // testing usability of full packages
-  let table = Pkg.mem_alloc #(i:ip.Pkg.t{ip.Pkg.registered i}) (key ip) in
-  let q = pkg ip (fun (_:ip.Pkg.t) -> a) good_of_i table in
+  let u : info1 ip ha_of_i good_of_i 0 = {parent=r; alg=a; good=good_of_i 0} in
+  let u = coerce_eq2 (info1 ip ha_of_i good_of_i) (Pkg.Pkg?.info q) u in
 
   let h0 = Mem.get() in
   // assert(
@@ -351,7 +293,7 @@ let test
   // assume(Monotonic.RRef.m_sel h0 (Pkg.itable table) == MM.empty_map ip.Pkg.t (key ip));
   // assert(MM.fresh (Pkg.itable table) 0 h0);
   // assert(q.Pkg.define_table == table);
-  assume(Pkg.mem_fresh q.Pkg.define_table 0 h0);
+  assume(mem_fresh q.Pkg.define_table 0 h0);
 
   //17-11-23  causing mysterious squash error
   // assert_by_tactic(u:info{u.alg = ha_of_i 0 /\ u.good == good_of_i 0} == Pkg.Pkg?.info q 0) FStar.Tactics.(norm "foo");
